Finish fixes to exchanger

Examples/NameSpec.v
@@ -1,13 +1,23 @@
 From LHL.Core Require Import
   Program
   ProgramFacts
+  Tensor
   Specs
-  Logic.
+  LogicPaco
+  Logic
+  LogicFacts
+  ProgramRules.
 
 From LHL.Util Require Import
   Tactics
   TransUtil
   Util.
+
+From Paco Require Import paco.
+
+From Coq Require Import
+  Logic.FunctionalExtensionality
+  Logic.PropExtensionality.
 
 Variant NameSig {T} : ESig :=
 | Self : NameSig (Name T).
@@ -27,32 +37,267 @@ Program Definition nameSpec {T} : Spec T (NameSig T) := {|
 
 Admit Obligations.
 
+Lemma trimProg {E A B} :
+  forall (C : Prog E B) (v : A),
+  (Return v;; C) = C.
+intros.
+rewrite frobProgId at 1. simpl.
+destruct C; easy.
+Qed.
+
+Lemma simpProg {E A B} :
+  forall (C : A -> Prog E B) (v : A),
+  (x <- Return v; C x) = C v.
+intros.
+rewrite frobProgId at 1. simpl.
+destruct C; easy.
+Qed.
+
+CoInductive selfProgWF {E P R} (C : P -> Prog E R) := {
+  returnWF :
+    forall x v,
+      C x = Return v ->
+      forall y, exists w,
+        C y = Return w /\
+        (x = y -> v = w);
+  bindWF :
+    forall x A (m1 : E A) k1,
+      C x = Bind m1 k1 ->
+      forall y, exists (m2 : P -> E A) k2,
+        C y = Bind (m2 y) (k2 y) /\
+        m1 = m2 x /\
+        k1 = k2 x /\
+        (forall z, selfProgWF (fun i' => k2 i' z));
+  noopWF :
+    forall x k1,
+      C x = NoOp k1 ->
+      forall y, exists k2,
+        C y = NoOp (k2 y) /\
+        k1 = k2 x /\
+        selfProgWF k2
+}.
+
 Lemma lemBindSelf {T E F A} {VE : Spec T E} {VF : Spec T F}
-  `{SigCoercion (NameSig T) E}
-  {P R G : Relt VE VF} {Q : Post VE VF A} {C : Name T -> Prog E A} :
+  {P R G : Relt (tensorSpec nameSpec VE) VF}
+  {Q : Post (tensorSpec nameSpec VE) VF A}
+  {C : Name T -> Prog (NameSig T |+| E) A} :
+  selfProgWF C ->
   forall i : Name T,
   VerifyProg i R G P (_ <- call Self; C i) Q ->
   VerifyProg i R G P (i' <- call Self; C i') Q.
-intros. ddestruct H0.
+intros WF. intros. ddestruct H.
 {
   rewrite frobProgId with (p:=_;;_) in x.
   simpl in x. ddestruct x.
 }
-{
+2:{
   rewrite frobProgId with (p:=_;;_) in x.
   simpl in x. ddestruct x.
-  rewrite frobProgId at 1. cbn.
-  eapply SafeBind with (QI:=QI) (QR:=QR).
-  easy. easy. easy.
-  intros. specialize (H3 i). destruct H3.
-  split.
+}
+rewrite frobProgId with (p:=_;;_) in x.
+simpl in x. ddestruct x.
+rewrite frobProgId at 1. cbn.
+eapply SafeBind with
+  (QI:=QI)
+  (QR:=fun v s xs t ys => i = v /\ QR v s xs t ys).
+easy.
+{
+  unfold Stable, stablePost, stableRelt, sub, subRelt.
+  intros. psimpl. split. easy.
+  apply H0. psplit. exact H5. easy.
+}
+easy.
+intros. specialize (H2 v). destruct H2.
+split.
+{
+  clear - H2.
+  unfold Commit in *. intros.
+  cbn in *. destruct H3. ddestruct H3.
+  cut (
+    exists σs : Poss VF -> Prop,
+    (exists σ : Poss VF, σs σ) /\
+    (forall σ : Poss VF, σs σ -> exists ρ : Poss VF, ρs ρ /\ PossSteps ρ σ) /\
+    QR i s ρs t σs /\ G s ρs t σs
+  ).
   {
-    clear - H3.
-    unfold Commit in *. intros.
-    admit.
+    intros. psimpl. exists x1.
+    split. exists x2. easy.
+    easy.
+  }
+  eapply H2. all: try easy.
+  rewrite <- x0, <- x.
+  repeat (easy || constructor).
+}
+{
+  rewrite trimProg in H3.
+  rewrite simpProg.
+  clear - H3 WF.
+  revert H3.
+  cut (
+    forall C P P',
+    selfProgWF C ->
+    (P' ==> P) ->
+    SafeProg i R G P (C i) Q ->
+    SafeProg i R G
+    (fun s xs t ys => i = v /\ P' s xs t ys) (C v) Q
+  ).
+  {
+    intros. eapply weakenPrec.
+    eapply H with
+      (P:= P ->> QI ->> QR v)
+      (P':= P ->> QI ->> QR v).
+    easy. easy.
+    exact H3.
+    unfold sub, subRelt.
+    intros. psimpl.
+    split. easy.
+    psplit. exact H0.
+    psplit. exact H1.
+    easy.
+  }
+  clear. setoid_rewrite paco_eqv.
+  pcofix rec. intros C P P' WF imp.
+  intros H0. punfold H0. ddestruct H0;
+  pfold; symmetry in x; destruct WF.
+  {
+    apply returnWF0 with (y:=v) in x.
+    psimpl. rewrite H0.
+    constructor. unfold sub, subRelt.
+    intros. psimpl.
+    specialize (H1 eq_refl). subst.
+    apply H, imp. easy.
   }
   {
-    admit.
+    apply bindWF0 with (y:=v) in x.
+    destruct x as [m' [k']].
+    psimpl. rewrite H3.
+    econstructor.
+    { exact H. }
+    { exact H0. }
+    {
+      unfold Commit. intros. psimpl.
+      eapply H1.
+      {
+        exists x, x0.
+        apply imp. easy.
+      }
+      { easy. }
+      { easy. }
+      { easy. }
+    }
+    {
+      intros.
+      specialize (H2 v0).
+      split.
+      {
+        unfold Commit. intros. psimpl.
+        eapply H2.
+        {
+          exists x, x0. psplit.
+          apply imp. exact H11.
+          easy.
+        }
+        { easy. }
+        { easy. }
+        { easy. }
+      }
+      {
+        right.
+        assert (
+          ((fun s xs t ys => i = v /\ P' s xs t ys) ->> QI ->> QR v0) =
+          (fun s xs t ys => i = v /\ (P' ->> QI ->> QR v0) s xs t ys)
+        ).
+        {
+          extensionality s. extensionality xs.
+          extensionality t. extensionality ys.
+          apply propositional_extensionality.
+          split; intros; psimpl.
+          {
+            split. easy.
+            psplit. exact H8.
+            psplit. exact H7.
+            easy.
+          }
+          {
+            psplit.
+            split. easy.
+            exact H5.
+            psplit.
+            exact H8.
+            easy.
+          }
+        }
+        rewrite H4 at 1.
+        eapply rec with (C:=fun i' => k' i' v0).
+        { apply H6. }
+        2:{
+          psimpl.
+          pclearbot. exact u.
+        }
+        {
+          unfold sub, subRelt.
+          intros. psimpl.
+          psplit. apply imp. exact H5.
+          psplit. exact H8.
+          easy.
+        }
+      }
+    }
+  }
+  {
+    apply noopWF0 with (y:=v) in x.
+    psimpl. rewrite H2.
+    econstructor.
+    { exact H. }
+    {
+      unfold SilentStep.
+      intros. psimpl.
+      eapply H0.
+      {
+        exists x0, x1.
+        now apply imp.
+      }
+      { easy. }
+      { easy. }
+    }
+    {
+      right.
+      assert (
+        ((fun s xs t ys => i = v /\ P' s xs t ys) ->> QS) =
+        (fun s xs t ys => i = v /\ (P' ->> QS) s xs t ys)
+      ).
+      {
+        extensionality s. extensionality xs.
+        extensionality t. extensionality ys.
+        apply propositional_extensionality.
+        split; intros; psimpl.
+        {
+          split. easy.
+          psplit. exact H6.
+          easy.
+        }
+        {
+          psplit.
+          split. easy.
+          exact H5.
+          easy.
+        }
+      }
+      rewrite H3.
+      eapply rec with (P:= P ->> QS).
+      { easy. }
+      {
+        unfold sub, subRelt.
+        intros. psimpl.
+        psplit. apply imp. exact H5.
+        easy.
+      }
+      {
+        pclearbot.
+        unfold paco_safe.
+        easy.
+      }
+    }
   }
 }
-Admitted.
+Qed.
